lean/privacy/notes/discoverable.lean
@@ -7,29 +7,39 @@ import privacy.notes.notes
 import privacy.notes.contiguous
 import privacy.notes.scanned_note
 
-----------------------------------
--- Scan notes for (channel, i₀) --
-----------------------------------
+structure ScanNoteContext (crypto: Crypto) (m: Memory) extends ScanTokenContext crypto m where
+  h_notes: ∀ c token i₀, ∃ i₁, m .Notes [crypto.hash [c, token, i₀, i₁], 0] = 0
 
-def scan_notes_for_channel_i₀
-    (crypto: Crypto) (rm: ReachableMemory crypto) (c token i₀: ℕ)
-    : List ScannedNote :=
-  have h_exists : ∃ i₁, rm.m .Notes [crypto.hash [c, token, i₀, i₁], 0] = 0 := by
+theorem ScanNoteContext.from {crypto: Crypto} (rm: ReachableMemory crypto) :
+    ScanNoteContext crypto rm := {
+  toScanTokenContext := .from rm,
+  h_notes := by
+    intro c token i₀
     obtain ⟨bound, h_bound⟩ := notes_contiguous c token i₀
     use bound
     have := (h_bound bound).not.mp (Nat.lt_irrefl bound)
     unfold note_exists at this
     simp only [ne_eq, not_not] at this
     exact this
-  let bound := Nat.find h_exists
+  }
+
+----------------------------------
+-- Scan notes for (channel, i₀) --
+----------------------------------
+
+def scan_notes_for_channel_i₀
+    {crypto: Crypto} {m: Memory} (context: ScanNoteContext crypto m)
+    (c token i₀: ℕ)
+    : List ScannedNote :=
+  let bound := Nat.find (context.h_notes c token i₀)
   (List.range bound).map (λ i₁ ↦ ⟨c, token, i₀, i₁⟩)
 
 -- Once a note is discoverable, it stays discoverable.
 theorem notes_discoverable_monotone {crypto: Crypto} {rm: ReachableMemory crypto} {action: Action}
-    (success: (run_action crypto action rm.m).2)
+    (success: (run_action crypto action rm.m).success)
     {c token i₀: ℕ} {sn: ScannedNote}
-    (h : sn ∈ scan_notes_for_channel_i₀ crypto rm c token i₀) :
-    sn ∈ scan_notes_for_channel_i₀ crypto (rm.add action success) c token i₀ := by
+    (h : sn ∈ scan_notes_for_channel_i₀ (.from rm) c token i₀) :
+    sn ∈ scan_notes_for_channel_i₀ (.from (rm.add action success)) c token i₀ := by
   simp only [scan_notes_for_channel_i₀, List.mem_map, List.mem_range, Nat.lt_find_iff] at *
   obtain ⟨i₁, h⟩ := h
   use i₁
@@ -45,12 +55,12 @@ theorem note_exists_implies_i₀
     (h_note_exists: note_exists rm note_id) :
     ∃ sn: ScannedNote,
       note_id = sn.note_id crypto ∧
-      sn ∈ scan_notes_for_channel_i₀ crypto rm sn.c sn.token sn.i₀ ∧
+      sn ∈ scan_notes_for_channel_i₀ (.from rm) sn.c sn.token sn.i₀ ∧
       sn.i₀ < crypto.MAX_I₀ ∧
       subchannel_exists crypto rm sn.c sn.token := by
   revert rm
   apply ReachableMemory.induction
-  case inv₀ => unfold note_exists; simp
+  case inv₀ => simp [note_exists, ReachableMemory.m]
 
   intro action rm ih success h_note_exists
   cases action
@@ -78,9 +88,7 @@ theorem note_exists_implies_i₀
           have : note_exists rm' (crypto.hash [inp.c crypto, inp.token, inp.i₀, inp.i₁]) := by
             -- TODO: can this be deduced from `note_exists`?
             simp [note_exists]
-            unfold rm' ReachableMemory.add run_action
-            simp
-            rw [←info.h_m']
+            rw [ReachableMemory.add_m, run_action, ←info.h_m']
             rw [info.memory_diff₀]
             exact crypto.pack_nz info.r_ne_zero
           obtain ⟨bound, h_bound⟩ := notes_contiguous (inp.c crypto) inp.token inp.i₀
@@ -95,8 +103,7 @@ theorem note_exists_implies_i₀
         exact info.subchannel_exists
     case neg =>
       have : note_id ≠ inp.note_id crypto := λ h₁ ↦ by simp [h₁] at h₀
-      simp only [ReachableMemory.add, run_action] at h_note_exists
-      rw [←info.h_m'] at h_note_exists
+      rw [ReachableMemory.add_m, run_action, ←info.h_m'] at h_note_exists
       rw [info.no_change _ _ (by simp [this]) (by simp)] at h_note_exists
       obtain ⟨⟨c, token, i₀, i₁⟩, ih₀, ih₁, ih₂, ih₃⟩ := ih h_note_exists
       use ⟨c, token, i₀, i₁⟩
@@ -114,19 +121,17 @@ theorem note_exists_implies_i₀
 ----------------------------
 
 def scan_notes_for_channel
-    (crypto: Crypto)
-    (rm: ReachableMemory crypto)
-    (c token: ℕ)
-    : List ScannedNote :=
+    {crypto: Crypto} {m: Memory} (context: ScanNoteContext crypto m)
+    (c token: ℕ) : List ScannedNote :=
   (List.range crypto.MAX_I₀).flatMap
-    λ i₀ ↦ scan_notes_for_channel_i₀ crypto rm c token i₀
+    λ i₀ ↦ scan_notes_for_channel_i₀ context c token i₀
 
 theorem scan_notes_for_channel_props {crypto: Crypto} {rm: ReachableMemory crypto}
     {sn: ScannedNote} {c token: ℕ}
-    (h: sn ∈ scan_notes_for_channel crypto rm c token) :
+    (h: sn ∈ scan_notes_for_channel (.from rm) c token) :
     sn.c = c ∧ sn.token = token := by
-  simp only [scan_notes_for_channel, scan_notes_for_channel_i₀, List.mem_flatMap, List.mem_range,
-    List.mem_map, Nat.lt_find_iff] at h
+  simp only [scan_notes_for_channel, scan_notes_for_channel_i₀,
+    List.mem_flatMap, List.mem_range, List.mem_map, Nat.lt_find_iff] at h
   obtain ⟨i₀, h_i₀, i₁, h₀, h₁⟩ := h
   simp [←h₁]
 
@@ -136,7 +141,7 @@ theorem note_exists_implies_for_channel (crypto: Crypto) (rm: ReachableMemory cr
     note_exists rm note_id →
     ∃ sn: ScannedNote,
     note_id = sn.note_id crypto ∧
-    sn ∈ scan_notes_for_channel crypto rm sn.c sn.token ∧
+    sn ∈ scan_notes_for_channel (.from rm) sn.c sn.token ∧
     subchannel_exists crypto rm sn.c sn.token := by
   intro note_id note_exists
   obtain ⟨sn, h₀, h₁, h₂, h₃⟩ := note_exists_implies_i₀ note_exists
@@ -151,22 +156,21 @@ theorem note_exists_implies_for_channel (crypto: Crypto) (rm: ReachableMemory cr
 ------------------------------
 
 def scan_notes_for_recipient
-    (crypto: Crypto)
-    (rm: ReachableMemory crypto)
+    {crypto: Crypto} {m: Memory} (context: ScanNoteContext crypto m)
     (addrbob: ℕ) (kbob: crypto.PrivateKeys)
     : List ScannedNote := do
-  let c ← scan_channels crypto rm addrbob kbob
-  let token ← scan_tokens_for_channel crypto rm c
-  scan_notes_for_channel crypto rm c token
+  let c ← scan_channels crypto m addrbob kbob
+  let token ← scan_tokens_for_channel (context.toScanTokenContext) c
+  scan_notes_for_channel context c token
 
 theorem scan_notes_for_recipient'
     (crypto: Crypto)
     (rm: ReachableMemory crypto)
     (sn: ScannedNote) (addrbob: ℕ) (kbob: crypto.PrivateKeys):
-    sn ∈ scan_notes_for_recipient crypto rm addrbob kbob ↔ (
+    sn ∈ scan_notes_for_recipient (.from rm) addrbob kbob ↔ (
       sn.c ∈ scan_channels crypto rm addrbob kbob ∧
-      sn.token ∈ scan_tokens_for_channel crypto rm sn.c ∧
-      sn ∈ scan_notes_for_channel crypto rm sn.c sn.token
+      sn.token ∈ scan_tokens_for_channel (.from rm) sn.c ∧
+      sn ∈ scan_notes_for_channel (.from rm) sn.c sn.token
     ) := by
   simp only [scan_notes_for_recipient, List.bind_eq_flatMap, List.mem_flatMap]
   constructor
@@ -185,24 +189,25 @@ theorem note_exists_implies_for_recipient
     {crypto: Crypto} {rm: ReachableMemory crypto} {note_id: ℕ}
     (h_note_exists: note_exists rm note_id) :
     ∃ addrbob : ℕ, ∃ kbob: crypto.PrivateKeys, ∃ sn: ScannedNote,
-      sn ∈ scan_notes_for_recipient crypto rm addrbob kbob ∧
+      sn ∈ scan_notes_for_recipient (.from rm) addrbob kbob ∧
       note_id = sn.note_id crypto ∧
+      channel_exists crypto rm sn.c ∧
       (∃ addralice kalice, sn.c = crypto.hash [addralice, kalice, addrbob, crypto.priv_to_pub kbob]) := by
   obtain ⟨sn, h_note_id, note_id_in_scan, subchannel_exists⟩ := note_exists_implies_for_channel crypto rm note_id h_note_exists
 
-  have := subchannel_exists_implies subchannel_exists
-  obtain ⟨addralice, kalice, addrbob, Kbob, h'⟩ := channels_are_discoverable this.2
+  have ⟨h_token, h_channel_exists⟩ := subchannel_exists_implies subchannel_exists
+  obtain ⟨addralice, kalice, addrbob, kbob, h'⟩ := channels_are_discoverable h_channel_exists
 
-  use addrbob, Kbob, sn
+  use addrbob, kbob, sn
   rw [scan_notes_for_recipient']
 
-  exact ⟨⟨h'.2, this.1, note_id_in_scan⟩, h_note_id, ⟨addralice, kalice, h'.1⟩⟩
+  exact ⟨⟨h'.2, h_token, note_id_in_scan⟩, h_note_id, h_channel_exists, ⟨addralice, kalice, h'.1⟩⟩
 
 -- Discoverable note → note_exists and c is linked to (addrbob, kbob).
 theorem discoverable_note_implies
     {crypto: Crypto} {rm: ReachableMemory crypto} {addrbob: ℕ} {kbob: crypto.PrivateKeys}
     {sn: ScannedNote}
-    (h: sn ∈ scan_notes_for_recipient crypto rm addrbob kbob) :
+    (h: sn ∈ scan_notes_for_recipient (.from rm) addrbob kbob) :
     note_exists rm (sn.note_id crypto) ∧
     (∃ addralice kalice, sn.c = crypto.hash [addralice, kalice, addrbob, crypto.priv_to_pub kbob]) := by
   rw [scan_notes_for_recipient'] at *
