lean/privacy/channels/discoverable_outgoing.lean
@@ -1,0 +1,139 @@
+import privacy.utils
+import privacy.actions
+import privacy.channels.channels
+import privacy.channels.contiguous
+
+structure ScanOutgoingChannelContext (crypto: Crypto) (m: Memory) where
+  h_outgoing_channels: ∀ addralice kalice, ∃ s, m .OutgoingChannels [crypto.hash [addralice, kalice, s], 0] = 0
+
+theorem ScanOutgoingChannelContext.from
+    {crypto: Crypto} (rm: ReachableMemory crypto)
+    : ScanOutgoingChannelContext crypto rm :=
+  {
+    h_outgoing_channels := by
+      intro addralice kalice
+      have ⟨bound, h_bound⟩ := outgoing_channels_contiguous rm addralice kalice
+      use bound
+      have := (h_bound bound).not.mp (Nat.lt_irrefl bound)
+      simp only [ne_eq, not_not] at this
+      exact this
+  }
+
+def scan_outgoing_channels
+    {crypto: Crypto} {m: Memory} (context: ScanOutgoingChannelContext crypto m)
+    (addralice kalice: ℕ) : List (ℕ × ℕ) :=
+  let bound := Nat.find (context.h_outgoing_channels addralice kalice)
+  (List.range bound).map (λ s ↦
+    let addrbob_enc := m .OutgoingChannels [crypto.hash [addralice, kalice, s], 1]
+    let Kbob_enc := m .OutgoingChannels [crypto.hash [addralice, kalice, s], 2]
+    let r := m .OutgoingChannels [crypto.hash [addralice, kalice, s], 0]
+    let sym_key_addrbob := crypto.hash [addralice, kalice, r, 0]
+    let sym_key_Kbob := crypto.hash [addralice, kalice, r, 1]
+
+    ⟨addrbob_enc - sym_key_addrbob, Kbob_enc - sym_key_Kbob⟩
+  )
+
+theorem scan_outgoing_channels_monotone
+   {crypto: Crypto} {rm: ReachableMemory crypto} {addralice kalice: ℕ}
+   {action: Action}
+   {item: ℕ × ℕ}
+   (success: (run_action crypto action rm).success)
+   (h: item ∈ scan_outgoing_channels (.from rm) addralice kalice) :
+   item ∈ scan_outgoing_channels (.from (rm.add action success)) addralice kalice := by
+  cases action
+  case CreateChannel inp =>
+    let info := create_channel_info crypto inp rm success
+    simp only [scan_outgoing_channels, List.mem_map, List.mem_range,
+      Nat.lt_find_iff, ReachableMemory.add_m, run_action, ←info.h_m'] at h ⊢
+    obtain ⟨s_bound, h₀, h₁⟩ := h
+    use s_bound
+
+    constructor
+    · intro s h_s_le_s_bound
+      have h_ne': crypto.hash [addralice, kalice, s] ≠ inp.outgoing_channel_id crypto := by
+        by_contra h_is_same
+        have := h₀ s h_s_le_s_bound
+        have := info.outgoing_channel_didnt_exist
+        rw [←h_is_same] at this
+        contradiction
+      rw [info.no_change _ _ (by simp [h_ne'])]
+      exact h₀ s h_s_le_s_bound
+    · have h_ne: crypto.hash [addralice, kalice, s_bound] ≠ inp.outgoing_channel_id crypto := by
+        by_contra h_is_same
+        have := h₀ s_bound (by rfl)
+        have := info.outgoing_channel_didnt_exist
+        rw [←h_is_same] at this
+        contradiction
+
+      rw [info.no_change _ _ (by simp [h_ne])]
+      rw [info.no_change _ _ (by simp [h_ne])]
+      rw [info.no_change _ _ (by simp [h_ne])]
+      exact h₁
+  all_goals exact h
+
+-----------------------------------------
+-- Channel exists implies discoverable --
+-----------------------------------------
+
+-- Channel exists → it is discoverable by scanning the outgoing channels.
+theorem outgoing_channels_are_discoverable {crypto: Crypto} {rm: ReachableMemory crypto}
+    {addralice kalice addrbob Kbob: ℕ}
+    (c_exists: channel_exists crypto rm (crypto.hash [addralice, kalice, addrbob, Kbob])) :
+    (addrbob, Kbob) ∈ scan_outgoing_channels (.from rm) addralice kalice := by
+  revert rm
+  apply ReachableMemory.induction
+  case inv₀ => simp [channel_exists, ReachableMemory.m]
+
+  intro action rm ih success c_exists
+  cases action
+  case CreateChannel inp =>
+    by_cases h_channel_existed: channel_exists crypto rm (crypto.hash [addralice, kalice, addrbob, Kbob])
+    case pos =>
+      -- Channel existed before.
+      exact scan_outgoing_channels_monotone success (ih h_channel_existed)
+    case neg =>
+      have ⟨inp, h_inp, h_c⟩ := channel_exists_iff_CreateChannel.1 c_exists
+
+      cases h_inp
+      case tail h_inp =>
+        have := channel_exists_iff_CreateChannel.2 ⟨inp, h_inp, h_c⟩
+        contradiction
+
+      -- Channel was just added.
+      let info := create_channel_info crypto inp rm success
+      simp only [scan_outgoing_channels, List.mem_map, List.mem_range,
+        Nat.lt_find_iff, ReachableMemory.add_m, run_action, ←info.h_m']
+      use inp.s
+
+      have : addralice = inp.addralice ∧ kalice = inp.kalice ∧ addrbob = inp.addrbob ∧ Kbob = inp.Kbob := by
+        apply crypto.h_hash at h_c
+        injections
+        simp [*]
+
+      constructor
+      · intro s' h_s'
+        have ⟨sbound, h_contiguous⟩ := outgoing_channels_contiguous rm addralice kalice
+
+        by_cases h_s'': s' = inp.s
+        case pos =>
+          simp only [h_s'', this, info.memory_diff₃]
+          exact info.r_ne_zero
+        case neg =>
+          cases info.prev_outgoing_exists
+          case inl h_prev => omega
+          case inr h_prev =>
+            have := (h_contiguous (inp.s - 1)).2 (by simp only [this]; exact h_prev)
+            have := (h_contiguous s').1 (by omega)
+
+            have h_ne : crypto.hash [addralice, kalice, s'] ≠ inp.outgoing_channel_id crypto := by
+              by_contra h_eq
+              apply crypto.h_hash at h_eq
+              injections h_eq
+              contradiction
+
+            rw [info.no_change _ _ (by simp [h_ne])]
+            exact this
+
+      · simp [this, info.memory_diff₃, info.memory_diff₄, info.memory_diff₅]
+
+  all_goals exact ih c_exists
