lean/privacy/subchannels/subchannels.lean
@@ -14,13 +14,12 @@ theorem subchannel_hash_exists_implies_hash
   cases action
   case CreateSubchannel inp =>
     let info := create_subchannel_info crypto inp rm success
-    dsimp only [ReachableMemory.add, run_action]
-    rw [←info.h_m']
+    rw [ReachableMemory.add_m, run_action, ←info.h_m']
     intro h'
 
     by_cases h_is_same: crypto.hash [c, addrbob, Kbob, token] = crypto.hash [inp.c, inp.addrbob, inp.Kbob, inp.token]
     case pos =>
-      obtain ⟨kalice, h_inp_c⟩ := channel_exists_implies_hash info.channel_exists
+      obtain ⟨kalice, h_inp_c⟩ := (channel_exists_implies_hash info.channel_exists).1
       apply crypto.h_hash at h_is_same
       injections
       use inp.addralice, kalice
@@ -38,20 +37,19 @@ def subchannel_exists (crypto: Crypto) (m: Memory) (c token: ℕ) : Prop :=
 -- Once a subchannel exists, it stays this way.
 theorem subchannel_exists_monotone
     {crypto: Crypto} {rm: ReachableMemory crypto} {action: Action}
-    (success: (run_action crypto action rm.m).2)
+    (success: (run_action crypto action rm.m).success)
     {c token: ℕ}
     (h : subchannel_exists crypto rm c token) :
     subchannel_exists crypto (rm.add action success) c token
 := by
-  unfold subchannel_exists ReachableMemory.add run_action
+  unfold subchannel_exists
   cases action
   case CreateSubchannel inp =>
     obtain ⟨addrbob, Kbob, h⟩ := h
     use addrbob, Kbob
-    simp only
 
     let info := create_subchannel_info crypto inp rm success
-    rw [←info.h_m']
+    rw [ReachableMemory.add_m, run_action, ←info.h_m']
 
     by_cases h_is_same : crypto.hash [c, addrbob, Kbob, token] = inp.subchannel_hash crypto
     case pos =>
