lean/privacy/transactions/transaction0.lean
@@ -1,0 +1,304 @@
+import privacy.utils
+import privacy.actions
+import privacy.transactions.immutability
+
+structure Transaction₀ where
+  actions: List Action
+
+structure RunTransactionActionResult where
+  m_s: Memory
+  m_c: Memory
+  events: List Event
+  success: Bool
+
+def run_transaction_action (crypto: Crypto) (action: Action) (inp: RunTransactionActionResult) : RunTransactionActionResult :=
+  -- Run the client-side.
+  let ⟨server_actions, success_c⟩ := run_action₀ crypto action inp.m_c
+  -- "Server"-side `success` of `run_all` on `m_c` is ignored.
+  let ⟨m_c, _⟩ := ServerAction.run_all crypto server_actions inp.m_c
+
+  -- Run the server-side.
+  let ⟨m_s, success_s⟩ := ServerAction.run_all crypto server_actions inp.m_s
+
+  let events' := inp.events ++get_events server_actions
+
+  { m_s := m_s, m_c := m_c, events := events', success := inp.success && success_c && success_s }
+
+def run_transaction_actions (crypto: Crypto) (actions: List Action) (m_s m_c: Memory) : RunTransactionActionResult :=
+  actions.foldr (run_transaction_action crypto) { m_s := m_s, m_c := m_c, events := [], success := true }
+
+theorem run_transaction_actions_cons₁ (crypto: Crypto) (action: Action) (actions: List Action) (m_s m_c: Memory) :
+    (run_transaction_actions crypto (action :: actions) m_s m_c).m_s =
+    let res := run_transaction_actions crypto actions m_s m_c
+    (ServerAction.run_all crypto (run_action₀ crypto action res.m_c).1 res.m_s).1 := by
+  rw [run_transaction_actions, run_transaction_actions, List.foldr_cons, run_transaction_action]
+
+theorem run_transaction_actions_cons₂ (crypto: Crypto) (action: Action) (actions: List Action) (m_s m_c: Memory) :
+    (run_transaction_actions crypto (action :: actions) m_s m_c).m_c =
+    let res := run_transaction_actions crypto actions m_s m_c
+    (ServerAction.run_all crypto (run_action₀ crypto action res.m_c).1 res.m_c).1 := by
+  rw [run_transaction_actions, run_transaction_actions, List.foldr_cons, run_transaction_action]
+
+theorem run_transaction_actions_cons₃ (crypto: Crypto) (action: Action) (actions: List Action) (m_s m_c: Memory) :
+    (run_transaction_actions crypto (action :: actions) m_s m_c).success =
+    let res := run_transaction_actions crypto actions m_s m_c
+    let client_success := (run_action₀ crypto action res.m_c).2
+    let server_success := (ServerAction.run_all crypto (run_action₀ crypto action res.m_c).1 res.m_s).2
+    res.success && client_success && server_success := by
+  rw [run_transaction_actions, run_transaction_actions, List.foldr_cons, run_transaction_action]
+
+theorem run_transaction_actions_m_c
+    (crypto: Crypto) (actions: List Action) (m_s m_c: Memory) :
+    (run_transaction_actions crypto actions m_s m_c).m_c =
+    (run_all crypto actions m_c).m := by
+  induction actions
+  case nil => simp [run_transaction_actions]
+  case cons action actions ih =>
+    rw [run_transaction_actions, List.foldr_cons, ←run_transaction_actions, run_transaction_action]
+    dsimp only
+    rw [run_all_cons₁, ih]
+    rfl
+
+theorem run_transaction_actions_events
+    (crypto: Crypto) (actions: List Action) (m_s m_c: Memory) :
+    (run_transaction_actions crypto actions m_s m_c).events =
+    (run_all crypto actions m_c).events := by
+  induction actions
+  case nil => simp [run_transaction_actions]
+  case cons action actions ih =>
+    rw [run_transaction_actions, List.foldr_cons, ←run_transaction_actions, run_transaction_action]
+    dsimp only
+    rw [run_all_cons_events, ih, List.append_cancel_left_eq]
+    rw [run_transaction_actions_m_c]
+    rfl
+
+-- A transaction and the "time" where the client-side ran.
+-- If `time=t`, it means that the client-side ran after the server-side execution of the first `t`
+-- transactions.
+structure TimedTransaction extends Transaction₀ where
+  time: ℕ
+
+structure RunTransactionsResult where
+  m: Memory
+  past_ms: List Memory
+  events: List (List Event)
+  success: Bool
+
+def run_transactions (crypto: Crypto) (ttxs: List TimedTransaction) : RunTransactionsResult :=
+  let initial_m: Memory := 0
+  ttxs.foldr (λ ttx res ↦
+    let res' := run_transaction_actions crypto ttx.actions res.m (res.past_ms[ttx.time]? |>.getD initial_m)
+    { m := res'.m_s, past_ms := res.past_ms ++ [res'.m_s], events := res.events ++ [res'.events], success := res.success && res'.success }
+  ) { m :=initial_m, past_ms := [initial_m], events := [], success := true }
+
+-------------------------
+
+theorem add_transaction_is_reachable
+    (crypto: Crypto) (actions: List Action) (rm_s rm_c: ReachableMemory crypto)
+    (h_extends: rm_s.extends rm_c) :
+    let res := run_transaction_actions crypto actions rm_s rm_c
+    res.success →
+    (∃ rm: ReachableMemory crypto,
+      rm.actions = actions ++ rm_s.actions ∧
+      rm.m = res.m_s ∧
+      rm.events = rm_s.events ++ res.events
+    ) ∧ (∃ server_actions: List ServerAction,
+      res.m_s = (ServerAction.run_all crypto server_actions rm_s).1 ∧
+      res.m_c = (ServerAction.run_all crypto server_actions rm_c).1
+    ) := by
+  induction actions
+  case nil =>
+    dsimp only
+    intro success
+    constructor
+    · use rm_s
+      simp [run_transaction_actions]
+    · use []
+      simp [run_transaction_actions, ServerAction.run_all]
+
+  case cons action actions ih =>
+    dsimp only
+    intro success
+    set res := run_transaction_actions crypto actions rm_s.m rm_c.m with h_res
+    set client_res := run_action₀ crypto action res.m_c with h_client_res
+
+    rw [run_transaction_actions_cons₃] at success
+    simp only [Bool.and_eq_true] at success
+    have success₀ : res.success := success.1.1
+    have success₁ : client_res.2 := success.1.2
+    have success₂ : (ServerAction.run_all crypto client_res.1 res.m_s).2 := success.2
+
+    obtain ⟨⟨rm, ih₀, ih₁, ih₂⟩, ⟨server_actions, ih₃, ih₄⟩⟩ := ih success₀
+    dsimp only at ih
+
+    have h_same_actions : run_action₀ crypto action res.m_s = client_res := by
+      let e: TransactionExecution := { m_c₀ := rm_c.m, m_s₀ := rm_s.m, actions := server_actions }
+      apply run_action₀_immutable (success:=success₁)
+
+      have h_extends' : rm.extends rm_c := by
+        have ⟨a, h⟩ := h_extends
+        use actions ++ a
+        simp [h, ih₀]
+
+      have := ImmutableCells.reflected_immutability' e (by
+        unfold TransactionExecution.m_s
+        rw [←ih₃, ←ih₁]
+        exact ImmutableCells.of_extends crypto h_extends'
+      )
+      rw [ih₃, ih₄]
+      exact this
+
+    constructor
+    · use rm.add action (by
+        rw [run_action, process_action, ih₁]
+        simp only [Bool.and_eq_true]
+        rw [h_same_actions]
+        exact ⟨success₁, success₂⟩
+      )
+      refine ⟨?_, ?_, ?_⟩
+      · simp [ih₀]
+      · rw [ReachableMemory.add_m, ih₁, run_transaction_actions_cons₁, run_action, process_action]
+        dsimp only
+        rw [h_same_actions]
+      · rw [ReachableMemory.add_events, ih₂]
+        rw [List.append_assoc, List.append_cancel_left_eq]
+        conv => rhs; rw [run_transaction_actions_events, run_all_cons_events]
+        rw [←run_transaction_actions_events (m_s:=rm_s.m)]
+        rw [List.append_cancel_left_eq]
+        dsimp only [run_action, process_action]
+        rw [ih₁, h_same_actions, h_client_res]
+        rw [run_transaction_actions_m_c]
+    · use server_actions ++ (run_action₀ crypto action res.m_s).1
+      constructor
+      · rw [run_transaction_actions_cons₁]
+        dsimp only
+        rw [ServerAction.run_all_append, ←h_res, ←ih₃, h_same_actions]
+      · rw [run_transaction_actions_cons₂]
+        dsimp only
+        rw [ServerAction.run_all_append, ←h_res, ←ih₄, h_same_actions]
+
+-------------------------
+
+theorem zero_in_past_ms
+    (crypto: Crypto) (ttxs: List TimedTransaction) :
+    0 ∈ (run_transactions crypto ttxs).past_ms := by
+  induction ttxs
+  case nil => simp [run_transactions]
+  case cons ttx ttxs ih =>
+    rw [run_transactions, List.foldr_cons, ←run_transactions]
+    dsimp only
+    rw [List.mem_append]
+    exact Or.inl ih
+
+theorem run_transactions_add_tx
+    (crypto: Crypto) (ttxs: List TimedTransaction) (ttx: TimedTransaction) :
+    let res₀ := run_transactions crypto ttxs
+    let res₁ := run_transactions crypto (ttx :: ttxs)
+    res₁.success →
+    res₀.success ∧
+    ∃ past_m ∈ res₀.past_ms,
+    res₁.m = (run_transaction_actions crypto ttx.actions res₀.m past_m).m_s ∧
+    res₁.events = res₀.events ++ [(run_transaction_actions crypto ttx.actions res₀.m past_m).events] ∧
+    (run_transaction_actions crypto ttx.actions res₀.m past_m).success := by
+  dsimp only
+  set res₀ := run_transactions crypto ttxs with h_res₀
+  set res₁ := run_transactions crypto (ttx :: ttxs) with h_res₁
+  intro success
+  unfold res₁ at success
+  rw [run_transactions, List.foldr_cons, ←run_transactions] at success
+  dsimp only at success
+  simp [Bool.and_eq_true] at success
+  have ⟨success₀, success₁⟩ := success
+  use success₀
+  use res₀.past_ms[ttx.time]?.getD 0
+  refine ⟨?_, ?_, ?_, ?_⟩
+  · by_cases h: ttx.time < res₀.past_ms.length
+    case pos => simp [List.getElem?_eq_getElem h]
+    case neg =>
+      rw [List.getElem?_eq_none (by omega)]
+      simp only [Option.getD_none]
+      apply zero_in_past_ms
+  · unfold res₁
+    rw [run_transactions, List.foldr_cons, ←run_transactions]
+  · unfold res₁
+    rw [run_transactions, List.foldr_cons, ←run_transactions]
+  · exact success₁
+
+theorem run_transactions_is_reachable
+    (crypto: Crypto) (ttxs: List TimedTransaction) :
+    let res := run_transactions crypto ttxs
+    res.success →
+    (∃ rm: ReachableMemory crypto,
+      rm.actions = ttxs >>= (λ ttx ↦ ttx.actions) ∧
+      rm.m = res.m ∧
+      rm.events = res.events.flatten ∧
+      (∀ past_m ∈ res.past_ms, ∃ past_rm: ReachableMemory crypto,
+        past_rm.m = past_m ∧ rm.extends past_rm
+      )
+    ) := by
+  intro res success
+  induction ttxs
+  case nil =>
+    use ReachableMemory.empty
+    refine ⟨?_, ?_, ?_, ?_⟩
+    · trivial
+    · trivial
+    · trivial
+    · unfold res
+      intro past_m h_past_m
+      use ReachableMemory.empty
+      simp only [run_transactions, List.foldr_nil, List.mem_cons, List.not_mem_nil, or_false] at h_past_m
+      rw [h_past_m]
+      constructor
+      · trivial
+      · exact ⟨[], by simp⟩
+  case cons ttx ttxs ih =>
+    unfold res at success
+    have ⟨success₀, past_m, h₀, h₁, h₂, h₃⟩ := run_transactions_add_tx crypto ttxs ttx success
+    have ⟨rm_s, ih₀, ih₁, ih_events, ih_past_ms⟩ := ih success₀
+    have ⟨past_rm, h_past_rm, h_extends⟩ := ih_past_ms past_m h₀
+    have ⟨⟨rm, h_rm_actions, h_rm_m, h_rm_events⟩, _⟩ := add_transaction_is_reachable crypto ttx.actions rm_s past_rm h_extends (by rwa [h_past_rm, ih₁])
+
+    have h_rm_m_eq_res1 : rm.m = res.m := by
+      unfold res
+      rw [h_rm_m, ih₁, h_past_rm, h₁]
+
+    use rm
+    refine ⟨?_, ?_, ?_, ?_⟩
+    · simp [h_rm_actions, ih₀]
+    · exact h_rm_m_eq_res1
+    · rw [h_rm_events]
+      rw [h₂, List.flatten_append, List.flatten_singleton]
+      rw [←ih_events, List.append_cancel_left_eq]
+      rw [ih₁, h_past_rm]
+    · intro past_m h_past_m
+      unfold res at h_past_m
+      rw [run_transactions, List.foldr_cons, ←run_transactions] at h_past_m
+      simp only [List.mem_append, List.mem_cons, List.not_mem_nil, or_false] at h_past_m
+      cases h_past_m
+      case inl h_past_m =>
+        have ⟨past_rm, h_past_rm_m, ⟨actions, h_actions⟩⟩ := ih_past_ms past_m h_past_m
+        refine ⟨past_rm, h_past_rm_m, ?_⟩
+        use ttx.actions ++ actions
+        simp [h_rm_actions, ←h_actions]
+      case inr h_past_m =>
+        rw [h_past_m]
+        exact ⟨rm, h_rm_m_eq_res1, [], by simp⟩
+
+theorem run_transactions_eq_run_sequentially
+    {crypto: Crypto} {ttxs: List TimedTransaction} :
+    let res := run_transactions crypto ttxs
+    let ⟨res_seq_m, res_seq_events, res_seq_success⟩ := run_all crypto (ttxs >>= (λ ttx ↦ ttx.actions)) 0
+    res.success → (
+      res.m = res_seq_m ∧
+      res.events.flatten = res_seq_events ∧
+      res.success = res_seq_success
+     ) := by
+  dsimp only
+  intro success
+  have ⟨rm, h₀, h₁, h₂, _⟩ := run_transactions_is_reachable crypto ttxs success
+  rw [←h₀, ←h₁, ←h₂]
+  refine ⟨?_, ?_, ?_⟩
+  · rw [ReachableMemory.m, h₀, run_all]
+  · rfl
+  · rw [success, rm.success]
